\documentclass[aspectratio=169]{ctexbeamer} %[t]：顶端对齐

\makeatletter
\def\input@path{{../../styles}}  % 
\makeatother
\usepackage{ubeamer}
\uBigPaper

\begin{document}

\begin{frame}[t]{完全立方公式及其证明}
完全立方公式有两个，分别是： \\
$(a + b)^3 = a^3 + 3a^2b + 3ab^2 + b^3$ \\
$(a - b)^3 = a^2 - 3a^2b + 3ab^2 - b^3$ \\
如何证明呢？
\vspace{0.5cm}
\begin{columns}
\column{0.5\textwidth}
\begin{flalign*} % 公式左对齐，需要收尾都有&字符。
\text{证明：}\\
&(a + b)^3 = (a + b)(a + b)(a+b) & \\
&=(a^2 + 2ab + b^2)(a+b) \\
&= a^3 + a^2b + 2a^2b + 2ab^2 + ab^2 + b^3&\\
&= a^3 + 3a^2b + 3ab^2 + b^3 &
\end{flalign*}
\column{0.5\textwidth}

\begin{flalign*} % 公式左对齐，需要收尾都有&字符。
\text{证明：}\\
&(a - b)^3 = (a-b)(a-b)(a-b) & \\
&=(a^2 - 2ab + b^2)(a - b) \\
&= a^3 - a^2b - 2a^2b + 2ab^2  + ab^2 - b^3&\\
&= a^3 - 3a^2b + 3ab^2 - b^3 &
\end{flalign*}
\end{columns}
\end{frame}

\end{document}
