\documentclass[aspectratio=169]{ctexbeamer} %[t]：顶端对齐

\makeatletter
\def\input@path{{../../styles}}  % 
\makeatother
\usepackage{ubeamer}
\uBigPaper

\begin{document}

\begin{frame}[t]{完全平方公式及其证明}
完全平方公式有两个，分别是： \\
$(a + b)^2 = a^2 + 2ab + b^2$ \\
$(a - b)^2 = a^2 - 2ab + b^2$ \\
如何证明呢？
\vspace{0.5cm}
\begin{columns}
\column{0.5\textwidth}
\begin{flalign*} % 公式左对齐，需要收尾都有&字符。
\text{证明：}\\
&(a + b)^2 = (a + b)(a + b) & \\
&=a(a+b) + b(a+b) \\
&= a^2 + ab + ba + b^2 &\\
&= a^2 + ab + ab + b^2 & \\
&= a^2 + 2ab + b^2 &
\end{flalign*}
\column{0.5\textwidth}

\begin{flalign*} % 公式左对齐，需要收尾都有&字符。
\text{证明：}\\
&(a - b)^2 = (a - b)(a - b) & \\
&=a(a - b) - b(a - b) \\
&= a^2 - ab - ba + b^2 &\\
&= a^2 - ab - ab + b^2 & \\
&= a^2 - 2ab + b^2 &
\end{flalign*}
\end{columns}
\end{frame}

\end{document}
