\documentclass[aspectratio=169]{ctexbeamer} %[t]：顶端对齐

\makeatletter
\def\input@path{{../../styles}}  % 
\makeatother
\usepackage{ubeamer}
\uBigPaper

\date{\today}
\begin{document}

\begin{frame}[t]{1.9 有理数的乘法}
\begin{spacing}{1.2}
\normalsize
有理数的乘法法则：
\begin{enumerate}[label={\arabic*.}]
\item 同号得正：$(-a) \cdot (-b)  = a  \cdot b$
\item 异号得负（绝对值相乘）：$(-a) \cdot b  = a  \cdot (-b) = -a \cdot b$
\item 乘零得零：$ a \cdot 0  =  0 \cdot a = 0$
\item 交换律：$a \cdot b \cdot c = a  \cdot c \cdot b = b  \cdot c \cdot a$
\item 结合律：$(a \cdot b) \cdot c = a \cdot (b \cdot c)$
\item 分配律：$a \cdot (b + c) = a \cdot b + a \cdot c$
\end{enumerate}

\end{spacing}
\end{frame}

\begin{frame}[t]{1.9 有理数的乘法}
\begin{spacing}{1.2}
\normalsize
有理数的乘法法则：
\begin{enumerate}[label={\arabic*.}]
\item 同号得正：$(-a)(-b)  = ab$
\item 异号得负（绝对值相乘）：$(-a)b  = a(-b) = -ab$
\item 乘零得零：$ a \cdot 0  =  0a = 0$
\item 交换律：$abc = acb = bca$
\item 结合律：$(ab)c = a(bc)$
\item 分配律：$a(b + c) = ab + ac$
\end{enumerate}

\end{spacing}
\end{frame}

\end{document}